updating concurrency machinery
Still need to fix forward_spawn. See atomics/verif_lock and progs64/verif_incr for examples of how much nicer it is to use Iris directly.

atomics/verif_lock.v
@@ -1,17 +1,22 @@
+Require Export iris_ora.logic.cancelable_invariants.
 Require Import VST.concurrency.conclib.
 Require Import VST.floyd.library.
 Require Import VST.atomics.SC_atomics.
 Require Import VST.concurrency.lock_specs.
 Require Import VST.concurrency.threads.
 
+Section mpred.
+
+Context `{!VSTGS Espec Σ, !cinvG Σ}.
+
 #[export] Program Instance atom_impl : atomic_int_impl := { atomic_int := Tstruct _atom_int noattr }.
 Next Obligation. Admitted.
 Next Obligation. Admitted.
 Next Obligation. Admitted.
-Axiom atomic_int_isptr : forall sh v p, atomic_int_at sh v p |-- !! isptr p.
-#[export] Hint Resolve atomic_int_isptr : saturate_local.
-Axiom atomic_int_timeless : forall sh v p, fupd.timeless' (atomic_int_at sh v p).
-#[export] Hint Resolve atomic_int_timeless : core.
+Axiom atomic_int_isptr : forall sh v p, atomic_int_at sh v p ⊢ ⌜isptr p⌝.
+#[local] Hint Resolve atomic_int_isptr : saturate_local.
+Axiom atomic_int_timeless : forall sh v p, Timeless (atomic_int_at sh v p).
+#[export] Existing Instance atomic_int_timeless.
 
 #[global] Opaque atomic_int_at.
 
@@ -25,74 +30,51 @@ Section PROOFS.
   Definition atom_store_spec := DECLARE _atom_store atomic_store_spec.
   Definition atom_CAS_spec := DECLARE _atom_CAS atomic_CAS_spec.
 
-  Definition inv_for_lock v R := EX b, atomic_int_at Ews (Val.of_bool b) v * if b then emp else R.
+  Definition inv_for_lock v R := ∃ b, atomic_int_at Ews (Val.of_bool b) v ∗ if b then emp else R.
 
-  Lemma inv_for_lock_nonexpansive : forall v, nonexpansive (inv_for_lock v).
-  Proof.
-    intros.
-    apply @exists_nonexpansive; intros.
-    apply sepcon_nonexpansive; [apply const_nonexpansive|].
-    destruct x; [apply const_nonexpansive | apply identity_nonexpansive].
-  Qed.
+  #[global] Instance inv_for_lock_nonexpansive : forall v, NonExpansive (inv_for_lock v).
+  Proof. solve_proper. Qed.
 
-  Definition atomic_lock_inv sh h R := let '(v, i, g) := h in !!(sh <> Share.bot /\ isptr v) && cinvariant i g (inv_for_lock v R) * cinv_own g sh.
+  Definition atomic_lock_inv sh h R := let '(v, i, g) := h in ⌜isptr v⌝ ∧ cinv i g (inv_for_lock v R) ∗ cinv_own g sh.
 
-  #[export] Program Instance atomic_impl : lock_impl := { t_lock := Tstruct _atom_int noattr; lock_handle := val * invariants.iname * ghosts.gname;
+  #[export] Program Instance atomic_impl : lock_impl := { t_lock := Tstruct _atom_int noattr; lock_handle := val * namespace * gname;
     ptr_of h := let '(v, i, g) := h in v; lock_inv := atomic_lock_inv }.
   Next Obligation.
   Proof.
-    unfold atomic_lock_inv.
-    apply sepcon_nonexpansive, const_nonexpansive.
-    apply @conj_nonexpansive; [apply const_nonexpansive|].
-    apply cinvariant_nonexpansive2, inv_for_lock_nonexpansive.
+    solve_proper.
   Qed.
   Next Obligation.
   Proof.
     unfold atomic_lock_inv.
-    destruct (isptr_dec v).
-    rewrite !prop_true_andp; auto.
-    rewrite <- !sepcon_assoc, (sepcon_comm (_ * cinv_own _ _)), !sepcon_assoc.
-    unfold cinv_own at 1 2; erewrite <- own_op by eauto.
-    rewrite <- sepcon_assoc; f_equal.
-    symmetry; apply cinvariant_dup.
-    { split; auto; intros ?; subst. apply join_Bot in H1 as []; contradiction. }
-    { rewrite prop_false_andp, !FF_sepcon, prop_false_andp, FF_sepcon; auto; intros []; contradiction. }
+    intros ?? ((?, ?), ?) ?.
+    rewrite /cinv_own own_op; iSplit.
+    - iIntros "(($ & $ & $) & (_ & _ & $))".
+    - iIntros "(#$ & #$ & $ & $)".
   Qed.
   Next Obligation.
   Proof.
-    unfold exclusive_mpred, atomic_lock_inv; Intros.
-    unfold cinv_own; sep_apply own_op'.
-    Intros ?; Intros.
-    apply sepalg.join_self, identity_share_bot in H0; contradiction.
-  Qed.
-  Next Obligation.
-  Proof.
+    intros ? ((?, ?), ?) ?.
     unfold atomic_lock_inv; entailer!.
   Qed.
 
-  (* We can use self_part sh h * R instead of selflock sh h R. *)
+  (* We can use self_part sh h ∗ R instead of selflock sh h R. *)
   Definition self_part sh (h : lock_handle) := let '(v, i, g) := h in cinv_own g sh.
 
-  Lemma self_part_exclusive : forall sh h, sh <> Share.bot -> exclusive_mpred (self_part sh h).
+(*  Lemma self_part_exclusive : forall sh h, sh <> Share.bot -> exclusive_mpred (self_part sh h).
   Proof.
     intros; unfold exclusive_mpred, self_part; destruct h as ((?, ?), ?).
     unfold cinv_own; rewrite own_op'; Intros ?.
     apply sepalg.join_self, identity_share_bot in H0; contradiction.
-  Qed.
+  Qed.*)
 
-  Lemma self_part_eq : forall sh1 sh2 h R, sh2 <> Share.bot -> lock_inv sh1 h (self_part sh2 h * R) * self_part sh2 h =
-    lock_inv sh1 h (self_part sh2 h * R) * lock_inv sh2 h (self_part sh2 h * R).
+  Lemma self_part_eq : forall sh1 sh2 h R, lock_inv sh1 h (self_part sh2 h ∗ R) ∗ self_part sh2 h ⊣⊢
+    lock_inv sh1 h (self_part sh2 h ∗ R) ∗ lock_inv sh2 h (self_part sh2 h ∗ R).
   Proof.
     intros.
     simpl; unfold atomic_lock_inv; destruct h as ((?, ?), ?).
-    destruct (eq_dec sh1 Share.bot).
-    { rewrite prop_false_andp, !FF_sepcon; auto; intros []; contradiction. }
-    destruct (isptr_dec v).
-    rewrite !prop_true_andp by auto.
-    unfold self_part at 2; rewrite cinvariant_dup at 1.
-    rewrite <- !sepcon_assoc; f_equal.
-    rewrite (sepcon_comm (_ * _) (cinvariant _ _ _)), <- sepcon_assoc; reflexivity.
-    { rewrite prop_false_andp, !FF_sepcon; auto; intros []; contradiction. }
+    iSplit.
+    - iIntros "((#$ & #$ & $) & $)".
+    - iIntros "(($ & $ & $) & (_ & _ & $))".
   Qed.
 
   Definition makelock_spec := DECLARE _makelock makelock_spec.
@@ -110,113 +92,72 @@ Section PROOFS.
     start_function.
     forward_call (vint 1).
     Intros p.
-    viewshift_SEP 0 (EX i g, lock_inv Tsh (p, i, g) (R (p, i, g))).
-    { go_lower; simpl.
-      entailer!.
-      eapply derives_trans, fupd_mono; [|apply exp_derives; intros; apply exp_derives; intros; apply sepcon_derives, derives_refl; apply andp_right, derives_refl; entailer!].
-      eapply derives_trans, cinv_alloc_dep.
-      unfold inv_for_lock.
-      do 2 (apply allp_right; intros).
-      eapply derives_trans, now_later.
-      Exists true; simpl; cancel. apply derives_refl. }
-    simpl.
+    viewshift_SEP 0 (∃ i g, lock_inv 1 (p, i, g) (R (p, i, g))).
+    { go_lowerx.
+      iIntros "(? & _)".
+      iDestruct (atomic_int_isptr with "[$]") as "#$".
+      iMod (cinv_alloc_strong (λ _, True%type) _ (nroot .@ "lock")) as (?) "(_ & ? & inv)".
+      { apply pred_infinite_True. }
+      iExists _, _; iFrame; iApply "inv".
+      rewrite /inv_for_lock.
+      iExists true; auto. }
     forward.
-    simpl; Exists (p, i, g); unfold atomic_lock_inv; entailer!.
+    Exists (p, i, g); unfold atomic_lock_inv; entailer!.
   Qed.
-
-  #[local] Hint Resolve Ensembles.Full_intro : core.
 
   Lemma body_freelock: semax_body Vprog Gprog f_freelock freelock_spec.
   Proof.
     start_function.
     destruct h as ((p, i), g); simpl; Intros.
-    gather_SEP (cinvariant _ _ _) (cinv_own _ _); viewshift_SEP 0 (cinvariant i g (inv_for_lock p R) * |> inv_for_lock p R).
-    { go_lower; simpl; Intros.
-      rewrite cinvariant_dup at 1; unfold cinvariant at 1; sep_apply (inv_open Ensembles.Full_set); auto.
-      eapply derives_trans, fupd_elim; [apply fupd_frame_r|].
-      rewrite later_orp, !distrib_orp_sepcon; apply orp_left.
-      - sep_apply (modus_ponens_wand' (cinv_own g Tsh)).
-        { apply orp_right2, now_later. }
-        sep_apply fupd_frame_r; rewrite emp_sepcon.
-        sep_apply fupd_frame_r; rewrite sepcon_comm; apply derives_refl.
-      - eapply derives_trans, except_0_fupd.
-        apply orp_right1.
-        rewrite sepcon_assoc; eapply derives_trans; [apply sepcon_derives, now_later; apply derives_refl|].
-        rewrite <- later_sepcon; apply later_derives.
-        sep_apply cinv_own_excl.
-        rewrite FF_sepcon; auto. }
+    gather_SEP (cinv _ _ _) (cinv_own _ _); viewshift_SEP 0 (cinv i g (inv_for_lock p R) ∗ ▷ inv_for_lock p R).
+    { go_lowerx.
+      iIntros "((#$ & ?) & _)".
+      iMod (cinv_cancel with "[$] [$]") as "$"; done. }
     unfold inv_for_lock at 2.
-    rewrite (later_exp' _ true); Intros b.
+    rewrite bi.later_exist; Intros b.
     destruct b.
-    - assert_PROP (is_pointer_or_null p) by entailer!.
-      forward_call (p).
+    - forward_call (p).
       { Exists (Val.of_bool true); cancel. }
       entailer!.
-      rewrite <- emp_sepcon; apply sepcon_derives, andp_left2, derives_refl.
-      apply inv_dealloc.
+      by iIntros "(_ & _)".
     - gather_SEP 0 1 2 3.
-      viewshift_SEP 0 FF.
-      go_lower.
-      rewrite cinvariant_dup at 1.
-      unfold cinvariant at 1; sep_apply (inv_open Ensembles.Full_set); auto.
-      eapply derives_trans, fupd_elim; [apply fupd_frame_r|].
-      rewrite <- !sepcon_assoc, (sepcon_comm _ (|> _)), <- !sepcon_assoc.
-      rewrite 3sepcon_assoc; eapply derives_trans; [apply sepcon_derives, derives_refl|].
-      { rewrite <- later_sepcon; apply later_derives.
-        rewrite distrib_orp_sepcon2; apply orp_left, derives_refl.
-        unfold inv_for_lock; Intros b.
-        sep_apply atomic_int_conflict; auto.
-        rewrite FF_sepcon; apply FF_left. }
-      rewrite <- !sepcon_assoc, (sepcon_comm _ (_ -* _)).
-      rewrite !later_sepcon, <- !sepcon_assoc, 4sepcon_assoc.
-      eapply derives_trans; [apply sepcon_derives; [apply derives_refl|]|].
-      rewrite <- !sepcon_assoc; eapply derives_trans, modus_ponens_wand.
-      eapply sepcon_derives, derives_trans; [|apply now_later | rewrite later_andp, later_wand; apply andp_left1, derives_refl].
-      rewrite !later_sepcon; entailer!.
-      { rewrite sepcon_assoc, <- later_sepcon, sepcon_FF.
-        eapply derives_trans; [apply sepcon_derives, derives_refl; apply now_later|].
-        rewrite <- later_sepcon, sepcon_FF.
-        eapply derives_trans, except_0_fupd; apply orp_right1; auto. }
-      { eapply semax_pre, semax_ff; entailer!. }
+      viewshift_SEP 0 (False : mpred).
+      go_lowerx.
+      iIntros "((#I & (p & R) & P & HR) & _)".
+      rewrite {1}/cinv.
+      iInv "I" as "[(% & p' & ?) | Hown]".
+      { iAssert (▷False) with "[p p']" as ">[]".
+        iApply atomic_int_conflict; last iFrame; auto. }
+      iAssert (▷ False) with "[-]" as ">[]".
+      iNext; rewrite bi.affinely_elim; iDestruct ("HR" with "[$P $R $Hown]") as "[]"; done.
+      { eapply semax_pre, semax_ff; go_lower; done. }
   Qed.
 
   Lemma body_release: semax_body Vprog Gprog f_release release_spec.
   Proof.
     start_function.
-    forward_call (ptr_of h, vint 0, @Ensembles.Full_set invariants.iname, @Ensembles.Empty_set invariants.iname, Q).
-    - simpl; unfold atomic_lock_inv; destruct h as ((p, i), g); Intros.
+    forward_call (ptr_of h, vint 0, ⊤ : coPset, ∅ : coPset, Q).
+    - destruct h as ((p, i), g); simpl; Intros.
       subst Frame; instantiate (1 := []); simpl; cancel.
-      rewrite cinvariant_dup at 1.
-      sep_apply (cinv_open Ensembles.Full_set); auto.
-      repeat sep_apply fupd_frame_r; apply fupd_elim.
-      rewrite prop_true_andp by auto.
-      sep_apply (modus_ponens_wand (cinvariant i g (inv_for_lock p R) * cinv_own g sh * P)).
-      unfold inv_for_lock at 1.
-      rewrite (later_exp' _ true); Intros b; destruct b.
-      + rewrite sepcon_emp, !sepcon_assoc; sep_eapply fupd_timeless; auto; repeat sep_eapply fupd_frame_r; apply fupd_elim.
-        sep_apply atomic_int_at__.
-        eapply derives_trans, fupd_mask_intro_all; rewrite <- wand_sepcon_adjoint.
-        Exists Ews; simpl; entailer!.
-        rewrite <- wand_sepcon_adjoint.
-        sep_apply fupd_frame_l; repeat sep_apply fupd_frame_r; apply fupd_elim.
-        unfold ptr_of; sep_apply (modus_ponens_wand' (R * atomic_int_at Ews (vint 0) p)).
-        { unfold inv_for_lock.
-          eapply derives_trans, now_later.
-          Exists false; cancel. }
-        repeat sep_apply fupd_frame_r; apply fupd_mono; cancel.
-        apply andp_left2; auto.
-      + eapply derives_trans, except_0_fupd; apply orp_right1.
-        rewrite sepcon_comm, !sepcon_assoc; eapply derives_trans; [apply sepcon_derives, now_later; apply derives_refl|].
-        rewrite <- later_sepcon; apply later_derives.
-        sep_apply weak_exclusive_conflict.
-        rewrite FF_sepcon; auto.
-    - hnf; inversion 1.
+      iIntros "((((HR & #I) & ?) & P) & HQ)".
+      iInv i as "((% & >p & ?) & Hown)" "Hclose".
+      destruct b.
+      + iExists Ews; rewrite (bi.pure_True (writable_share _)) //.
+        rewrite atomic_int_at__; iFrame.
+        iApply fupd_mask_intro; first set_solver.
+        iIntros "Hmask p".
+        iDestruct ("HQ" with "[$Hown $P]") as "($ & ?)"; first auto.
+        iMod "Hmask"; iApply "Hclose".
+        iExists false; iFrame.
+      + iDestruct ("HQ" with "[$Hown $P]") as "(? & ?)"; first auto.
+        iAssert (▷ False) with "[-]" as ">[]".
+        rewrite bi.affinely_elim; iNext; iApply ("HR" with "[$]").
     - entailer!.
   Qed.
 
   Lemma body_acquire: semax_body Vprog Gprog f_acquire acquire_spec.
   Proof.
-    start_function; simpl.
+    start_function.
     forward.
     forward_loop (PROP ( )
                        LOCAL (temp _b (vint 0); lvar _expected tint v_expected;
@@ -225,72 +166,52 @@ Section PROOFS.
     { entailer!. }
     forward.
     forward_call
-      (ptr_of h, Tsh, v_expected, (vint 0), (vint 1), @Ensembles.Full_set invariants.iname, @Ensembles.Empty_set invariants.iname,
+      (ptr_of h, Tsh, v_expected, (vint 0), (vint 1), ⊤ : coPset, ∅ : coPset,
             fun v':val =>
-              atomic_lock_inv sh h R * if (eq_dec v' (vint 0)) then |> R else emp).
+              atomic_lock_inv sh h R ∗ if (eq_dec v' (vint 0)) then ▷ R else emp).
     - unfold atomic_lock_inv; destruct h as ((p, i), g); Intros.
       subst Frame; instantiate (1 := []); simpl fold_right_sepcon; cancel.
-      rewrite cinvariant_dup at 1.
-      sep_apply (cinv_open Ensembles.Full_set); auto.
-      repeat sep_apply fupd_frame_r; apply fupd_elim.
-      unfold inv_for_lock at 1.
-      rewrite (later_exp' _ true); Intros b.
-      rewrite later_sepcon; sep_eapply fupd_timeless; auto; repeat sep_eapply fupd_frame_r; apply fupd_elim.
-      eapply derives_trans, fupd_mask_intro_all; rewrite <- wand_sepcon_adjoint.
-      Exists Ews (Val.of_bool b); simpl; entailer!.
-      rewrite <- wand_sepcon_adjoint.
-      sep_apply fupd_frame_l; repeat sep_apply fupd_frame_r; apply fupd_elim.
-      destruct b; simpl eq_dec.
-      + rewrite !if_false by discriminate.
-        sep_eapply fupd_timeless; [apply fupd.emp_timeless|]; repeat sep_eapply fupd_frame_r; apply fupd_elim.
-        rewrite emp_sepcon.
-        sep_apply (modus_ponens_wand' (atomic_int_at Ews (Val.of_bool true) p)).
-        { unfold inv_for_lock.
-          eapply derives_trans, now_later.
-          Exists true; cancel. }
-        repeat sep_apply fupd_frame_r; apply fupd_mono; cancel.
-      + rewrite !if_true by auto.
-        sep_apply (modus_ponens_wand' (atomic_int_at Ews (vint 1) p)).
-        { unfold inv_for_lock.
-          eapply derives_trans, now_later.
-          Exists true; cancel. }
-        repeat sep_apply fupd_frame_r; apply fupd_mono; cancel.
-    - hnf; inversion 1.
+      iIntros "(#I & ?)".
+      iInv "I" as "((% & >? & ?) & ?)" "Hclose".
+      iExists Ews, (Val.of_bool b); rewrite (bi.pure_True (writable_share _)) //.
+      iFrame.
+      iApply fupd_mask_intro; first set_solver.
+      iIntros "Hmask p"; iMod "Hmask" as "_".
+      destruct b; simpl.
+      + iMod ("Hclose" with "[-]"); last auto.
+        iExists true; iFrame.
+      + iMod ("Hclose" with "[p]"); last by iFrame; auto.
+        iExists true; iFrame; auto.
     - Intros r. if_tac; forward_if; try discriminate; try contradiction.
-      + forward. simpl lock_specs.lock_inv; entailer!.
-      + forward. simpl lock_specs.lock_inv; entailer!.
+      + forward. simpl lock_inv; entailer!.
+      + forward. simpl lock_inv; entailer!.
   Qed.
 
 End PROOFS.
+
+Opaque lock_inv.
 
 (* freelock and release specialized for self_part *)
 Program Definition freelock_spec_self :=
   TYPE (ProdType (ConstType _) Mpred)
   WITH sh1 : _, sh2 : _, h : _, R : _
   PRE [ tptr t_lock ]
-     PROP (sh2 <> Share.bot; sepalg.join sh1 sh2 Tsh)
+     PROP (sh1 ⋅ sh2 = 1%Qp)
      PARAMS (ptr_of h)
-     SEP (lock_inv sh1 h (self_part sh2 h * R); self_part sh2 h)
+     SEP (lock_inv sh1 h (self_part sh2 h ∗ R); self_part sh2 h)
   POST [ tvoid ]
      PROP ()
      LOCAL ()
      SEP ().
 Next Obligation.
 Proof.
-  repeat intro.
-  destruct x as (((?, ?), ?), ?); simpl.
-  unfold PROPx, PARAMSx, GLOBALSx, LOCALx, SEPx, argsassert2assert; simpl; rewrite !approx_andp; do 3 f_equal;
-    rewrite -> !sepcon_emp, ?approx_sepcon, ?approx_idem.
-  f_equal.
-  setoid_rewrite (@lock_inv_super_non_expansive atomic_impl); do 2 f_equal.
-  rewrite !approx_sepcon, approx_idem; auto.
+  intros ? (((?, ?), ?), ?) (((?, ?), ?), ?) ([=] & HR) ?; simpl in *; subst.
+  by repeat f_equiv.
 Qed.
 Next Obligation.
 Proof.
-  repeat intro.
-  destruct x as (((?, ?), ?), ?); simpl.
-  unfold PROPx, LOCALx, SEPx; simpl; rewrite !approx_andp; do 2 f_equal;
-    rewrite -> !sepcon_emp, ?approx_sepcon, ?approx_idem.
+  intros ? (((?, ?), ?), ?) (((?, ?), ?), ?) ([=] & HR) ?; simpl in *; subst.
+  by repeat f_equiv.
 Qed.
 
 Program Definition release_spec_self :=
@@ -299,73 +220,68 @@ Program Definition release_spec_self :=
   PRE [ tptr t_lock ]
      PROP ()
      PARAMS (ptr_of h)
-     SEP (lock_inv sh h (self_part sh h * R); R)
+     SEP (<affine> (R ∗ R -∗ False); lock_inv sh h (self_part sh h ∗ R); R)
   POST [ tvoid ]
      PROP ()
      LOCAL ()
      SEP ().
 Next Obligation.
 Proof.
-  repeat intro.
-  destruct x as ((?, ?), ?); simpl.
-  unfold PROPx, PARAMSx, GLOBALSx, LOCALx, SEPx, argsassert2assert; simpl; rewrite !approx_andp; do 3 f_equal;
-    rewrite -> !sepcon_emp, ?approx_sepcon, ?approx_idem.
-  f_equal.
-  setoid_rewrite (@lock_inv_super_non_expansive atomic_impl); do 2 f_equal.
-  rewrite !approx_sepcon, approx_idem; auto.
+  intros ? ((?, ?), ?) ((?, ?), ?) ([=] & HR) ?; simpl in *; subst.
+  by repeat f_equiv.
 Qed.
 Next Obligation.
 Proof.
-  repeat intro.
-  destruct x as ((?, ?), ?); simpl.
-  reflexivity.
+  intros ? ((?, ?), ?) ((?, ?), ?) ([=] & HR) ?; simpl in *; subst.
+  by repeat f_equiv.
 Qed.
 
-#[export] Hint Resolve self_part_exclusive : core.
+Transparent lock_inv.
 
 Lemma release_self : funspec_sub lock_specs.release_spec release_spec_self.
 Proof.
   unfold funspec_sub; simpl.
-  split; auto; intros ? ((sh, h), R) ?; Intros.
-  eapply derives_trans, fupd_intro.
-  Exists (nil : list Type) (sh, h, self_part sh h * R, R, emp) emp; entailer!.
-  { intros; unfold PROPx, LOCALx, SEPx; simpl; entailer!. }
-  unfold atomic_lock_inv; destruct h as ((?, ?), ?).
-  unfold PROPx, PARAMSx, GLOBALSx, LOCALx, SEPx, argsassert2assert; simpl; entailer!.
-  lock_props.
-  { fold (self_part sh (v, i, g)); apply exclusive_sepcon1; auto. }
-  rewrite <- sepcon_emp at 1; apply sepcon_derives; [apply now_later|].
-  rewrite <- wand_sepcon_adjoint, emp_sepcon; cancel.
-  apply inv_dealloc.
+  split; first done; intros ((sh, h), R) ?; Intros.
+  iIntros "(? & ? & H) !>"; iExists (sh, h, self_part sh h ∗ R, R, emp), emp.
+  iSplit.
+  - repeat (iSplit; first done).
+    rewrite /SEPx /= /LOCALx /argsassert2assert /=; monPred.unseal.
+    repeat (iSplit; first done).
+    iDestruct "H" as "(? & HR & ? & ? & _)"; iFrame.
+    iSplitL "HR".
+    + iIntros "!> ((? & ?) & (? & ?))".
+      rewrite bi.affinely_elim; iApply ("HR" with "[$]").
+    + iSplit; first done; iSplit; last done.
+      destruct h as ((?, ?), ?); iIntros "((% & (? & $)) & $)".
+  - iPureIntro; intros.
+    unfold PROPx, LOCALx, SEPx; simpl; entailer!.
 Qed.
-
-Lemma lock_inv_share : forall sh h R, lock_inv sh h R |-- !!(sh <> Share.bot /\ isptr (ptr_of h)).
-Proof.
-  intros; destruct h as ((?, ?), ?); simpl; Intros; entailer!.
-Qed.
-
-#[export] Hint Resolve lock_inv_share : saturate_local.
 
 Lemma freelock_self : funspec_sub lock_specs.freelock_spec freelock_spec_self.
 Proof.
   unfold funspec_sub; simpl.
-  split; auto; intros ? (((sh1, sh2), h), R) ?; Intros.
-  eapply derives_trans, fupd_intro.
-  Exists (nil : list Type) (h, self_part sh2 h * R, emp) emp; entailer!.
-  { intros; unfold PROPx, LOCALx, SEPx; simpl; entailer!. }
-  unfold PROPx, PARAMSx, GLOBALSx, LOCALx, SEPx, argsassert2assert; simpl.
-  set (P := _ * _); entailer!; subst P.
-  rewrite sepcon_emp; setoid_rewrite self_part_eq; auto.
-  saturate_local.
-  erewrite lock_inv_share_join by eauto; simpl; cancel.
-  apply andp_right; auto.
-  rewrite <- wand_sepcon_adjoint, emp_sepcon.
-  destruct h as ((p, i), g); simpl; Intros.
-  sep_apply cinv_own_excl.
-  rewrite FF_sepcon; auto.
+  split; first done; intros (((sh1, sh2), h), R) ?; Intros.
+  iIntros "((%Hsh & _) & ? & H) !>"; iExists (h, self_part sh2 h ∗ R, emp), emp.
+  iSplit.
+  - repeat (iSplit; first done).
+    rewrite /SEPx /= /LOCALx /argsassert2assert /=; monPred.unseal.
+    repeat (iSplit; first done).
+    iDestruct "H" as "(? & p & self & _)"; iFrame.
+    iCombine "p self" as "p"; rewrite self_part_eq lock_inv_share_join Hsh; iFrame.
+    iSplit; first done; iSplit; last done.
+    iIntros "!> (_ & p & self & ?)".
+    iCombine "p self" as "p"; rewrite self_part_eq lock_inv_share_join.
+    destruct h as ((?, ?), ?); simpl.
+    iDestruct "p" as "(_ & _ & ? & ?)"; iApply (cinv_own_1_l with "[$] [$]").
+  - iPureIntro; intros.
+    unfold PROPx, LOCALx, SEPx; simpl; entailer!.
 Qed.
 
-Definition selflock R sh h := self_part sh h * R.
+Definition selflock R sh h := self_part sh h ∗ R.
+
+End mpred.
+
+#[export] Hint Resolve atomic_int_isptr : saturate_local.
 
 Opaque t_lock.
 Opaque lock_handle.
