progs64/io_specs.v
@@ -4,12 +4,7 @@ Require Export VST.floyd.io_events.
 Require Export ITree.ITree.
 Require Export ITree.Eq.
 Require Export ITree.Eq.SimUpToTaus.
-(* Import ITreeNotations. *) (* one piece conflicts with subp notation *)
-Notation "x <- t1 ;; t2" := (ITree.bind t1 (fun x => t2))
-  (at level 100, t1 at next level, right associativity) : itree_scope.
-Notation "' p <- t1 ;; t2" :=
-  (ITree.bind t1 (fun x_ => match x_ with p => t2 end))
-(at level 100, t1 at next level, p pattern, right associativity) : itree_scope.
+Import ITreeNotations.
 
 Definition stdin := 0%nat.
 Definition stdout := 1%nat.
